Der_encode_primitive skeleton; fix exec spec; incorporate der_write_tags  [skip ci]

src/Primitive/Prim/Der_encode_primitive.v
@@ -1,5 +1,5 @@
 Require Import Core.Core Lib.Lib Core.StructNormalizer 
-        VstLib Prim.Exec Lib.Callback.Dummy Lib.DWT.Vst.
+        VstLib Prim.Exec Lib.Callback.Dummy Lib.DWT.VST.Der_write_tags.
 Require Import VST.floyd.proofauto.
 Require Import Clight.dummy Clight.asn_codecs_prim.
 
@@ -8,14 +8,14 @@ Definition Vprog : varspecs. Proof. mk_varspecs prog. Defined.
 
 Section Der_encode_primitive.
 
-Definition prim_enc_rval td li sptr_p := 
-  match evalErrW (primitive_encoder td li) [] with
-  | Some v => mk_enc_rval v Vzero
-  | None => mk_enc_rval (-1) sptr_p
+Definition prim_enc_rval td sl buf_size li td_p sptr_p := 
+  match evalErrW (primitive_encoder td sl buf_size li) [] with
+  | Some v => mk_enc_rval v td_p Vzero
+  | None => mk_enc_rval (-1) td_p sptr_p
   end.
 
-Definition prim_enc_res td li := 
-  match execErrW (primitive_encoder td li) [] with
+Definition prim_enc_res td  sl buf_size li := 
+  match execErrW (primitive_encoder td  sl buf_size li) [] with
   | Some v => v
   | None => []
   end.
@@ -23,51 +23,71 @@ Definition prim_enc_res td li :=
 Definition prim_type_s := (Tstruct _ASN__PRIMITIVE_TYPE_s noattr).
 Definition mk_prim_type_s (buf_p : val) size := (buf_p, Vint (Int.repr size)).
 
+Instance Change1 : change_composite_env Callback.Dummy.CompSpecs CompSpecs.
+Proof. make_cs_preserve Dummy.CompSpecs CompSpecs. Defined.
+
+Instance Change2 : change_composite_env CompSpecs Dummy.CompSpecs.
+Proof. make_cs_preserve CompSpecs Dummy.CompSpecs. Defined.
+
+Instance Change4 : change_composite_env CompSpecs Der_write_tags.CompSpecs.
+Proof. make_cs_preserve CompSpecs Der_write_tags.CompSpecs. Defined.
+
+
+Instance Change3 : change_composite_env Der_write_tags.CompSpecs CompSpecs.
+Proof. make_cs_preserve Der_write_tags.CompSpecs CompSpecs. Defined.
+
 Definition der_primitive_encoder_spec : ident * funspec :=
   DECLARE _der_encode_primitive
     WITH res_p : val,  
          sptr_p : val, buf_b : block, buf_ofs : ptrofs, 
-         size : Z, data : list byte,
+         size : Z,
          td_p : val, td : TYPE_descriptor,
-         tag_mode : Z, tag : Z,
+         tag_mode : Z,
          cb_p : val, app_key_p : val
     PRE [tptr enc_rval_s, tptr type_descriptor_s, tptr tvoid, tint, tuint, 
           tptr cb_type, tptr tvoid]
-      PROP ()
+    PROP ( tag_mode = 0;
+             1 = Zlength (tags td);
+         0 <= size <= Int.max_unsigned)
       PARAMS (res_p; td_p; sptr_p; Vint (Int.repr tag_mode);
-              Vint (Int.repr tag); cb_p; app_key_p)
+              Vint (Int.repr 0); cb_p; app_key_p)
       GLOBALS ()
       SEP (data_at_ Tsh enc_rval_s res_p;
-           data_at_ Tsh type_descriptor_s td_p; 
            (* sptr *)
-           valid_pointer (Vptr buf_b buf_ofs);
-           if Val.eq (Vptr buf_b buf_ofs) nullval 
-           then emp
-           else data_at Tsh (tarray tuchar size) (map Vubyte data) (Vptr buf_b buf_ofs);
+           field_at Tsh (Tstruct der_encoder._asn_TYPE_descriptor_s noattr) 
+                    (DOT der_encoder._tags) (Vptr buf_b buf_ofs) td_p;
+           field_at Tsh (Tstruct der_encoder._asn_TYPE_descriptor_s noattr)
+                    (DOT der_encoder._tags_count) (Vint (Int.repr (Zlength (tags td)))) td_p;
+           data_at Tsh (tarray tuint (Zlength (tags td))) (map Vint (map Int.repr (tags td)))
+                   (Vptr buf_b buf_ofs);
            field_at Tsh prim_type_s (DOT _buf) (Vptr buf_b buf_ofs) sptr_p;
            field_at Tsh prim_type_s (DOT _size) (Vint (Int.repr size)) sptr_p;
            (* Callback *)
            data_at_ Tsh enc_key_s app_key_p;
+           func_ptr' dummy_callback_spec cb_p;
            valid_pointer cb_p)
     POST [tvoid]
+    let buf_size := if eq_dec cb_p nullval then 0 else 32 in
       PROP ()
       LOCAL ()
-      SEP (data_at_ Tsh type_descriptor_s td_p;
-           (* sptr *)
-           valid_pointer (Vptr buf_b buf_ofs);
-           if Val.eq (Vptr buf_b buf_ofs) nullval 
-           then emp
-           else data_at Tsh (tarray tuchar size) (map Vubyte (prim_enc_res td data)) 
-                        (Vptr buf_b buf_ofs);
-           data_at Tsh prim_type_s (mk_prim_type_s (Vptr buf_b buf_ofs) size) sptr_p;
+      SEP (field_at Tsh (Tstruct der_encoder._asn_TYPE_descriptor_s noattr) 
+                    (DOT der_encoder._tags) (Vptr buf_b buf_ofs) td_p;
+           field_at Tsh (Tstruct der_encoder._asn_TYPE_descriptor_s noattr)
+                    (DOT der_encoder._tags_count) (Vint (Int.repr (Zlength (tags td)))) td_p;
+           data_at Tsh  (tarray tuint (Zlength (tags td)))
+                   (map Vint (map Int.repr (tags td)))
+                   (Vptr buf_b buf_ofs);
+           field_at Tsh prim_type_s (DOT _buf) (Vptr buf_b buf_ofs) sptr_p;
+           field_at Tsh prim_type_s (DOT _size) (Vint (Int.repr size)) sptr_p;
            (* Result *)
-           data_at Tsh enc_rval_s (prim_enc_rval td data sptr_p) res_p;
+           data_at Tsh enc_rval_s (prim_enc_rval td size buf_size (map Int.repr (tags td))
+                                                 td_p sptr_p ) res_p;
            (* Callback *)
            valid_pointer cb_p;
            data_at_ Tsh enc_key_s app_key_p;
            func_ptr' dummy_callback_spec cb_p).
 
-Definition Gprog := ltac:(with_library prog [der_primitive_encoder_spec]).
+Definition Gprog := ltac:(with_library prog [der_primitive_encoder_spec; der_write_tags_spec]).
 
 Ltac forward_empty_loop :=
       match goal with
@@ -83,9 +103,86 @@ Proof.
   start_function. 
   forward.
   forward_empty_loop.
- (* forward_call (gv, td_p, td, 1, tag_mode, 0, tag, app_key_p, buf_b, buf_ofs, 
-                buf_size, computed_size, mem_size). *)
-
+  forward_call (td_p, td, size, 0, 0, cb_p, app_key_p, Vptr buf_b buf_ofs).
+  entailer!.
+  unfold Frame.
+  instantiate (1 := [data_at_ Tsh (Tstruct _asn_enc_rval_s noattr) v_erval ;
+                     data_at_ Tsh enc_rval_s res_p;
+                     field_at Tsh prim_type_s (DOT _buf) (Vptr buf_b buf_ofs) sptr_p ;
+                     field_at Tsh prim_type_s (DOT _size) (Vint (Int.repr size)) sptr_p ]).
+  simpl.
+  change_compspecs Der_write_tags.CompSpecs.
+  entailer!.
+  admit. (* change compspecs - same as in der_write_TL *)
+  repeat split; auto; try lia.
+  forward.
+  forward_empty_loop.
+  destruct (((Der_write_tags.der_write_tags td size 0 0 0
+                   (if Val.eq cb_p nullval then 0 else 32)) []
+              )) eqn : DWT. 
+  unfold evalErrW.
+  erewrite DWT.
+  forward_if.
+  - (* DWT returns -1 *)
+    repeat forward.
+    entailer!.
+    assert ((Vint (Int.repr (-1)), (td_p, sptr_p))  =
+            (prim_enc_rval td size (if eq_dec cb_p nullval then 0 else 32) 
+           (map Int.repr (tags td)) td_p sptr_p)) as P.
+    { unfold prim_enc_rval.
+      unfold evalErrW.
+      cbn.
+      break_if.
+      erewrite e0 in *.
+      erewrite if_true in DWT by auto.
+      erewrite DWT.
+      auto.
+      erewrite if_false in DWT by auto.
+      erewrite DWT.
+      auto. }
+    erewrite P.
+    entailer!.
+    admit. (* change compspecs - same as in der_write_TL *)
+  - discriminate.
+  - (* DWT returns a *)
+    unfold evalErrW.
+    erewrite DWT.
+    break_let.
+    forward_if.
+    admit. (* return not -1 - see lemma *) 
+    forward_if  [temp _t'11 (Vptr buf_b buf_ofs);
+                      temp _t'4 Vone].
+    + (* isptr cb *)
+      forward.
+      forward.
+      break_let.
+      entailer!.
+    + admit. (* cb_p = nullval *)
+    + forward_if [temp _t'9 (Vptr buf_b buf_ofs);
+                  temp _t'10  (Vint (Int.repr size));
+                  temp _t'2  Vzero]; try congruence.
+      *
+      repeat forward.
+      forward_call ((Vptr buf_b buf_ofs), size, app_key_p).
+      replace (size <? 0) with false by admit.
+      forward_if. congruence.
+      forward.
+      entailer!.
+      * discriminate.
+      *
+      repeat forward.
+      entailer!.
+      (* Int.min_signed <= Int.signed (Int.repr (encoded a)) + Int.signed (Int.repr size) <=
+  Int.max_signed *) admit.
+       match goal with
+      | [ _ : _ |- semax _ ?Pre _ _ ] =>
+          forward_loop Pre break: Pre 
+      end. 
+       entailer!.
+       repeat forward.
+       entailer!.
+       { admit. (* func correctness *) }
+       admit.
 Admitted.
 
 End Der_encode_primitive.
